

Conditional Probability

Conditional PMF (discrete case)

- ❖ The conditional PMF of X given that $Y = y$

$$p_{X|Y}(x|y) = P(X = x|Y = y) = \frac{P\{X = x, Y = y\}}{P(Y = y)} = \frac{p(x, y)}{p_Y(y)}$$

$$E[X|Y = y] = \sum_x xP\{X = x|Y = y\} = \sum_x xp_{X|Y}(x|y)$$

- ❖ (Example 3.1) $p(1,1) = 0.5$, $p(1,2) = 0.1$, $p(2,1) = 0.1$, $p(2,2) = 0.3$

- (Question) $p_{X|Y}(x|1) = ?$
- $p_Y(1) = \sum_x p(x, 1) = p(1,1) + p(2,1) = 0.6$
- $p_{X|Y}(1|1) = \frac{p(1,1)}{p_Y(1)} = \frac{0.5}{0.6}$, $p_{X|Y}(2|1) = \frac{p(2,1)}{p_Y(1)} = \frac{0.1}{0.6}$

Conditional PMF – Binomial

❖ (Example 3.2) $X_1 \sim \text{Binomial}(n_1, p)$, $X_2 \sim \text{Binomial}(n_2, p)$

- (Question) What is the conditional PMF of X_1 given $X_1 + X_2 = m$?
- (Solution) Let $q = 1 - p$

$$\begin{aligned} P(X_1 = k | X_1 + X_2 = m) &= \frac{P\{X_1=k, X_2=m-k\}}{P(X_1+X_2=m)} = \\ &= \frac{\binom{n_1}{k} p^k q^{n_1-k} \binom{n_2}{m-k} p^{m-k} q^{n_2-m+k}}{\binom{n_1+n_2}{m} p^m q^{n_1+n_2-m}} = \\ &= \frac{\binom{n_1}{k} \binom{n_2}{m-k}}{\binom{n_1+n_2}{m}} \rightarrow \text{hypergeometric distribution} \end{aligned}$$

Conditional PMF – Poisson

❖ (Example 3.3) $X_1 \sim \text{Poisson}(\lambda_1)$, $X_2 \sim \text{Poisson}(\lambda_2)$

- (Question) What is the conditional PMF of X_1 given $X_1 + X_2 = n$?

- (Solution)

$$P(X_1 = k | X_1 + X_2 = n) = \frac{P\{X_1 = k, X_2 = n - k\}}{P(X_1 + X_2 = n)} = \frac{P\{X_1 = k\}P\{X_2 = n - k\}}{P(X_1 + X_2 = n)}$$

Conditional PMF – Poisson

❖ (Example 2.37) $X_1 \sim \text{Poisson}(\lambda_1)$, $X_2 \sim \text{Poisson}(\lambda_2)$

$$\begin{aligned} P(X_1 + X_2 = n) &= \sum_{k=0}^n P\{X_1 = k, X_2 = n - k\} \\ &= \sum_{k=0}^n P\{X_1 = k\}P\{X_2 = n - k\} = \sum_{k=0}^n e^{-\lambda_1} \frac{\lambda_1^k}{k!} e^{-\lambda_2} \frac{\lambda_2^{n-k}}{(n-k)!} \\ &= e^{-\lambda_1} e^{-\lambda_2} \sum_{k=0}^n \frac{\lambda_1^k}{k!} \frac{\lambda_2^{n-k}}{(n-k)!} = \frac{e^{-(\lambda_1 + \lambda_2)}}{n!} \sum_{k=0}^n \frac{n!}{k! (n-k)!} \lambda_1^k \lambda_2^{n-k} \\ &= \frac{e^{-(\lambda_1 + \lambda_2)}}{n!} (\lambda_1 + \lambda_2)^n = \frac{(\lambda_1 + \lambda_2)^n}{n!} e^{-(\lambda_1 + \lambda_2)} \end{aligned}$$

i.e. $X_1 + X_2 \sim \text{Poisson}(\lambda_1 + \lambda_2)$

Conditional PMF – Poisson

❖ (Example 3.3) $X_1 \sim \text{Poisson}(\lambda_1)$, $X_2 \sim \text{Poisson}(\lambda_2)$

- (Question) What is the conditional PMF of X_1 given $X_1 + X_2 = n$?
- (Solution)

$$\begin{aligned} P(X_1 = k | X_1 + X_2 = n) &= \frac{P\{X_1 = k, X_2 = n - k\}}{P(X_1 + X_2 = n)} = \frac{P\{X_1 = k\}P\{X_2 = n - k\}}{P(X_1 + X_2 = n)} \\ &= \frac{e^{-\lambda_1} \frac{\lambda_1^k}{k!} e^{-\lambda_2} \frac{\lambda_2^{n-k}}{(n-k)!}}{\frac{(\lambda_1 + \lambda_2)^n}{n!} e^{-(\lambda_1 + \lambda_2)}} = \binom{n}{k} \left(\frac{\lambda_1}{\lambda_1 + \lambda_2}\right)^k \left(\frac{\lambda_2}{\lambda_1 + \lambda_2}\right)^{n-k} \end{aligned}$$

➔ Binomial $(n, \frac{\lambda_1}{\lambda_1 + \lambda_2})$

➔ $E[X_1 | X_1 + X_2 = n] = n \frac{\lambda_1}{\lambda_1 + \lambda_2}$